Show that Ne / Nf terms are a generic typing instance.
This is made possible by the fact that generic instances need not be
sound w.r.t. declarative typing now. We use this to alternatively prove
normalization in a straightforward way that does not require fancy
constructions.

theories/Normalisation.v
@@ -7,26 +7,161 @@ From LogRel Require Import LogicalRelation UntypedValues Validity Fundamental.
 From LogRel.LogicalRelation Require Import Escape Neutral Induction ShapeView Reflexivity.
 From LogRel.Substitution Require Import Escape Poly.
 
+Record WN (t : term) := {
+  wn_val : term;
+  wn_red : [ t ⇒* wn_val ];
+  wn_whnf : whnf wn_val;
+}.
+
+Lemma WN_wk : forall t (ρ : nat -> nat), WN t -> WN t⟨ρ⟩.
+Proof.
+intros * [r].
+exists r⟨ρ⟩.
++ now apply credalg_wk.
++ now apply whnf_ren.
+Qed.
+
+Lemma WN_exp : forall t u, [t ⇒* u] -> WN u -> WN t.
+Proof.
+intros t u ? [r].
+exists r; tea.
+now etransitivity.
+Qed.
+
+Lemma WN_whnf : forall t, whnf t -> WN t.
+Proof.
+intros; exists t; tea.
+reflexivity.
+Qed.
+
+Lemma WN_isFun : forall t, isFun t -> WN t.
+Proof.
+intros t []; apply WN_whnf; now constructor.
+Qed.
+
+Lemma WN_isPair : forall t, isPair t -> WN t.
+Proof.
+intros t []; apply WN_whnf; now constructor.
+Qed.
+
+Module Nf.
+
+Definition nf := de.
+
+#[export] Instance WfContextNf : WfContext nf := fun Γ => True.
+#[export] Instance WfTypeNf : WfType nf := fun Γ A => True.
+#[export] Instance TypingNf : Typing nf := fun Γ A t => True.
+#[export] Instance ConvTypeNf : ConvType nf := fun Γ A B => WN A × WN B.
+#[export] Instance ConvTermNf : ConvTerm nf := fun Γ A t u => WN t × WN u.
+#[export] Instance ConvNeuConvNf : ConvNeuConv nf := fun Γ A m n => whne m × whne n.
+#[export] Instance RedTypeNf : RedType nf := fun Γ A B => [A ⇒* B].
+#[export] Instance RedTermNf : RedTerm nf := fun Γ A t u => [t ⇒* u].
+
+#[export, refine] Instance WfCtxDeclProperties : WfContextProperties (ta := nf) := {}.
+Proof.
+all: try constructor.
+Qed.
+
+#[export, refine] Instance WfTypeDeclProperties : WfTypeProperties (ta := nf) := {}.
+Proof.
+all: try constructor.
+Qed.
+
+#[export, refine] Instance TypingDeclProperties : TypingProperties (ta := nf) := {}.
+Proof.
+all: try constructor.
+Qed.
+
+#[export, refine] Instance ConvTypeDeclProperties : ConvTypeProperties (ta := nf) := {}.
+Proof.
+all: try (intros; split; apply WN_whnf; now constructor).
++ intros * []; now split.
++ intros; split.
+  - intros t u []; now split.
+  - intros t u v [] []; now split.
++ intros * ? []; split; now apply WN_wk.
++ intros * ? ? []; split; now eapply WN_exp.
+Qed.
+
+#[export, refine] Instance ConvTermDeclProperties : ConvTermProperties (ta := nf) := {}.
+Proof.
+all: try (intros; split; apply WN_whnf; now constructor).
++ intros; split.
+  - intros t u []; now split.
+  - intros t u v [] []; now split.
++ intros * [] ?; now split.
++ intros * ? []; split; now apply WN_wk.
++ intros * ? ? ? []; split; now eapply WN_exp.
++ intros * []; split; now apply WN_whnf, whnf_whne.
++ intros * ? ? ? ? ? []; split; now apply WN_isFun.
++ intros; split; now apply WN_isPair.
+Qed.
+
+#[export, refine] Instance ConvNeuDeclProperties : ConvNeuProperties (ta := nf) := {}.
+Proof.
++ intros; split.
+  - intros t u []; now split.
+  - intros t u v [] []; now split.
++ intros * [] ?; now split.
++ intros * ? []; split; now apply whne_ren.
++ intros; split; constructor.
++ intros * [] ?; split; now constructor.
++ intros * ? ? ? []; split; now constructor.
++ intros * ? []; split; now constructor.
++ intros * []; split; now constructor.
++ intros * []; split; now constructor.
+Qed.
+
+#[export, refine] Instance RedTermDeclProperties : RedTermProperties (ta := nf) := {}.
+Proof.
+all: try now (intros; apply redalg_one_step; constructor).
++ intros; now apply credalg_wk.
++ intros; eassumption.
++ now constructor.
++ intros; now apply redalg_app.
++ intros; now apply redalg_natElim.
++ intros; now apply redalg_natEmpty.
++ intros; now apply redalg_fst.
++ intros; now apply redalg_snd.
++ intros; assumption.
++ intros; reflexivity.
+Qed.
+
+#[export, refine] Instance RedTypeDeclProperties : RedTypeProperties (ta := nf) := {}.
+Proof.
+all: try now intros; eassumption.
++ intros; now apply credalg_wk.
++ constructor.
++ intros; reflexivity.
+Qed.
+
+Export UntypedValues.WeakValuesProperties.
+
+#[export] Instance DeclarativeTypingProperties : GenericTypingProperties nf _ _ _ _ _ _ _ _ _ _ _ _ _ _ := {}.
+
+End Nf.
+
 Section Normalisation.
-  Context `{GenericTypingProperties}.
+
+  Import Nf.
 
   Theorem typing_nf : WfDeclInductionConcl
     (fun _ => True)
-    (fun Γ A => Nf[Γ |- A])
-    (fun Γ A t => Nf[Γ |- t : A])
-    (fun Γ A B => Nf[Γ |- A] × Nf[Γ |- B])
-    (fun Γ A t u => Nf[Γ |- t : A] × Nf[Γ |- u : A]).
+    (fun Γ A => True)
+    (fun Γ A t => True)
+    (fun Γ A B => WN A × WN B)
+    (fun Γ A t u => WN t × WN u).
   Proof.
     red.
     prod_splitter.
-    all: intros * []%Fundamental.
-    - easy.
-    - now eapply reifyType, reducibleTy.
-    - now eapply reifyTerm, reducibleTm.
-    - split.
-      all: now eapply reifyType, reducibleTy.
-    - split.
-      all: now eapply reifyTerm, reducibleTm.
+    all: intros * H%Fundamental.
+    - constructor.
+    - constructor.
+    - constructor.
+    - destruct H as [? ? ? H].
+      apply escapeEq in H as []; now split.
+    - destruct H as [? ? ? ? H].
+      apply escapeTmEq in H as []; now split.
   Qed.
 
 End Normalisation.
@@ -40,23 +175,28 @@ Theorem typing_SN Γ t :
   Acc cored t.
 Proof.
   intros [[] Hty].
-  all: eapply typing_nf in Hty as [? [red wh]].
+  all: first [apply TypeRefl in Hty|apply TermRefl in Hty].
+  all: eapply typing_nf in Hty as [? _].
+  all: pose proof w as [wh red].
   all: induction red.
   - econstructor.
     intros t' [red].
     exfalso.
     eapply whnf_nored ; tea.
-    now gen_typing.
   - econstructor.
     intros t'' [red'].
-    now eapply ored_det in red' as <-.
+    eapply ored_det in red' as <-; [|exact o].
+    apply IHred; tea.
+    eapply WN_exp; [tea|]; now apply WN_whnf.
   - econstructor.
     intros t' [red].
     exfalso.
     now eapply whnf_nored.
   - econstructor.
     intros t'' [red'].
-    now eapply ored_det in red' as <-. 
+    eapply ored_det in red' as <-; [|exact o].
+    apply IHred; tea.
+    eapply WN_exp; [tea|]; now apply WN_whnf.
 Qed.
 
 Section NeutralConversion.
